More proofs about CakeML itree semantics

cakeml-semantics/cakeml_semanticsProofScript.sml
@@ -1,9 +1,9 @@
 (* Relating the itree- and FFI state-based CakeML semantics *)
 open HolKernel Parse boolLib bossLib BasicProvers dep_rewrite;
-open optionTheory relationTheory pairTheory listTheory;
+open optionTheory relationTheory pairTheory listTheory arithmeticTheory;
 open lem_pervasives_extraTheory libTheory namespaceTheory astTheory
      ffiTheory semanticPrimitivesTheory smallStepTheory;
-open io_treeTheory cakeml_semanticsTheory;
+open io_treeTheory cakeml_semanticsTheory pure_miscTheory;
 
 val _ = new_theory "cakeml_semanticsProof";
 
@@ -24,12 +24,49 @@ val itree_ss = simpLib.named_rewrites "itree_ss" [
     cakeml_semanticsTheory.estep_def
     ];
 
+
+(****************************************)
+(* Copied from CakeML *)
+
+
+Theorem cml_application_thm:
+  ∀op env s vs c.
+    application op env s vs c =
+    if op = Opapp then
+      case do_opapp vs of
+      | NONE => Eabort Rtype_error
+      | SOME (env,e) => Estep (env,s,Exp e,c)
+    else
+      case do_app s op vs of
+      | NONE => Eabort Rtype_error
+      | SOME (v1,Rval v') => return env v1 v' c
+      | SOME (v1,Rerr (Rraise v)) => Estep (env,v1,Val v,(Craise (),env)::c)
+      | SOME (v1,Rerr (Rabort a)) => Eabort a
+Proof
+  rw[smallStepTheory.application_def] >> every_case_tac >> gvs[]
+QED
+
+
+(****************************************)
 (* Adapt CakeML's RTC definitions to our more functional definitions *)
+
+
 Definition step_n_cml_def:
   step_n_cml 0 e = e ∧
   step_n_cml (SUC n) (Estep st) = step_n_cml n (e_step st) ∧
   step_n_cml _ e = e
 End
+
+Theorem step_n_same[simp]:
+  ∀n.
+    step_n n Edone = Edone ∧
+    step_n n Etype_error = Etype_error ∧
+    step_n n (Effi s ws1 ws2 n env st cs) = (Effi s ws1 ws2 n env st cs) ∧
+    step_n_cml n Estuck = Estuck ∧
+    step_n_cml n (Eabort a) = Eabort a
+Proof
+  Cases >> rw[step_n_def, step_n_cml_def]
+QED
 
 Theorem step_n_cml_alt_def:
   step_n_cml 0 e = e ∧
@@ -43,6 +80,13 @@ Proof
   Induct >> Cases >> rewrite_tac[step_n_cml_def] >> simp[]
 QED
 
+Theorem step_n_cml_add:
+  ∀a b. step_n_cml (a + b) e = step_n_cml a (step_n_cml b e)
+Proof
+  Induct >> rw[step_n_cml_def] >>
+  simp[ADD_CLAUSES, step_n_cml_alt_def]
+QED
+
 Theorem e_step_reln_eq_step_n_cml:
   e_step_reln^* st1 st2 ⇔
   ∃n. step_n_cml n (Estep st1) = Estep st2
@@ -51,7 +95,7 @@ Proof
   >- (
     map_every qid_spec_tac [`st2`,`st1`,`n`] >>
     Induct >> rw[step_n_cml_alt_def] >>
-    EVERY_CASE_TAC >> gvs[] >>
+    every_case_tac >> gvs[] >>
     rw[Once relationTheory.RTC_CASES2] >> disj2_tac >>
     last_x_assum $ irule_at Any >> gvs[e_step_reln_def]
     )
@@ -70,13 +114,13 @@ Definition is_halt_cml_def:
 End
 
 Definition step_to_halt_cml_def:
-  step_to_halt_cml env st_ffi ev cs =
-    case some n. is_halt_cml (step_n_cml n (Estep (env, st_ffi, ev, cs))) of
+  step_to_halt_cml e =
+    case some n. is_halt_cml (step_n_cml n e) of
     | NONE => NONE
-    | SOME n => SOME $ step_n_cml n (Estep (env, st_ffi, ev, cs))
+    | SOME n => SOME $ step_n_cml n e
 End
 
-Theorem small_eval_eq_step_to_halt_cml:
+Theorem small_eval_eq_step_n_cml:
   (small_eval env st_ffi e cs (st_ffi', Rval v) ⇔
   ∃n env'.
     step_n_cml n (Estep (env, st_ffi, Exp e, cs)) =
@@ -94,7 +138,7 @@ Proof
     eq_tac >> rw[]
     >- (qexists_tac `SUC n` >> gvs[step_n_cml_alt_def]) >>
     Induct_on `n` >> gvs[step_n_cml_alt_def] >>
-    EVERY_CASE_TAC >> gvs[] >> rw[PULL_EXISTS] >>
+    every_case_tac >> gvs[] >> rw[PULL_EXISTS] >>
     PairCases_on `p` >> goal_assum drule >> simp[]
     ) >>
   eq_tac >> rw[] >> ntac 2 $ goal_assum drule
@@ -111,10 +155,109 @@ Proof
   simp[e_step_def, SF smallstep_ss]
 QED
 
+Triviality Estep_is_halt_imp_step_n_neq_Estep:
+  is_halt_cml st ⇒ ∀st'. step_n_cml (SUC n) st ≠ Estep st'
+Proof
+  Cases_on `st` >> gvs[is_halt_cml_def] >>
+  PairCases_on `p` >>
+  Cases_on `p3` >> gvs[is_halt_cml_def] >>
+  Cases_on `p4` >> gvs[is_halt_cml_def]
+  >- (gvs[step_n_cml_def, e_step_def, SF smallstep_ss, is_halt_cml_def]) >>
+  PairCases_on `h` >> Cases_on `h0` >> gvs[is_halt_cml_def] >>
+  Cases_on `t` >> gvs[is_halt_cml_def] >>
+  gvs[step_n_cml_def, e_step_def, SF smallstep_ss, is_halt_cml_def]
+QED
+
+Theorem small_eval_eq_step_to_halt_cml:
+  (small_eval env st_ffi e cs (st_ffi', Rval v) ⇔
+  ∃env'.
+    step_to_halt_cml (Estep (env, st_ffi, Exp e, cs)) =
+      SOME (Estep (env', st_ffi', Val v, []))) ∧
+  (small_eval env st_ffi e cs (st_ffi', Rerr (Rraise v)) ⇔
+  ∃env' env''.
+    step_to_halt_cml (Estep (env, st_ffi, Exp e, cs)) =
+      SOME (Estep (env', st_ffi', Val v, [(Craise (), env'')]))) ∧
+  ((∃st_ffi'. small_eval env st_ffi e cs (st_ffi', Rerr (Rabort a))) ⇔
+  ∃env' env''.
+    step_to_halt_cml (Estep (env, st_ffi, Exp e, cs)) = SOME (Eabort a))
+Proof
+  rw[small_eval_eq_step_n_cml, step_to_halt_cml_def] >> eq_tac >>
+  DEEP_INTRO_TAC some_intro >> rw[] >> gvs[]
+  >- (
+    Cases_on `n < x` >> gvs[]
+    >- (
+      `step_n_cml (SUC n) (Estep (env,st_ffi,Exp e, cs)) = Estuck` by (
+        simp[step_n_cml_alt_def, e_step_def, SF smallstep_ss]) >>
+      `∃p. x = p + SUC n` by (
+        imp_res_tac arithmeticTheory.LESS_STRONG_ADD >> gvs[ADD_CLAUSES]) >>
+      gvs[step_n_cml_add, is_halt_cml_def]
+      )
+    >- (
+      Cases_on `n = x` >> gvs[] >> `x < n` by gvs[] >>
+      imp_res_tac arithmeticTheory.LESS_STRONG_ADD >>
+      gvs[step_n_cml_add |> ONCE_REWRITE_RULE [Once ADD_COMM]] >>
+      gvs[Estep_is_halt_imp_step_n_neq_Estep]
+      )
+    )
+  >- (
+    pop_assum $ qspec_then `n` assume_tac >>
+    CCONTR_TAC >> gvs[is_halt_cml_def]
+    )
+  >- goal_assum drule
+  >- (
+    Cases_on `n < x` >> gvs[]
+    >- (
+      `step_n_cml (SUC n) (Estep (env,st_ffi,Exp e, cs)) = Estuck` by (
+        simp[step_n_cml_alt_def, e_step_def, SF smallstep_ss]) >>
+      `∃p. x = p + SUC n` by (
+        imp_res_tac arithmeticTheory.LESS_STRONG_ADD >> gvs[ADD_CLAUSES]) >>
+      gvs[step_n_cml_add, is_halt_cml_def]
+      )
+    >- (
+      Cases_on `n = x` >> gvs[] >> `x < n` by gvs[] >>
+      imp_res_tac arithmeticTheory.LESS_STRONG_ADD >>
+      gvs[step_n_cml_add |> ONCE_REWRITE_RULE [Once ADD_COMM]] >>
+      gvs[Estep_is_halt_imp_step_n_neq_Estep]
+      )
+    )
+  >- (
+    pop_assum $ qspec_then `n` assume_tac >>
+    CCONTR_TAC >> gvs[is_halt_cml_def]
+    )
+  >- goal_assum drule
+  >- (
+    Cases_on `n < x` >> gvs[]
+    >- (
+      `step_n_cml (SUC n) (Estep (env,st_ffi,Exp e, cs)) = Eabort a` by (
+        simp[step_n_cml_alt_def, e_step_def, SF smallstep_ss]) >>
+      `∃p. x = p + SUC n` by (
+        imp_res_tac arithmeticTheory.LESS_STRONG_ADD >> gvs[ADD_CLAUSES]) >>
+      gvs[step_n_cml_add, is_halt_cml_def]
+      )
+    >- (
+      Cases_on `n = x` >> gvs[] >> `x < n` by gvs[] >>
+      imp_res_tac arithmeticTheory.LESS_STRONG_ADD >>
+      gvs[step_n_cml_add |> ONCE_REWRITE_RULE [Once ADD_COMM]] >>
+      Cases_on `step_n_cml x (Estep (env,st_ffi,Exp e,cs))` >> gvs[is_halt_cml_def] >>
+      rename1 `_ $ Estep st` >> PairCases_on `st` >> gvs[step_n_cml_def] >>
+      Cases_on `st3` >> gvs[is_halt_cml_def] >>
+      Cases_on `st4` >> gvs[is_halt_cml_def, e_step_def, SF smallstep_ss] >>
+      PairCases_on `h` >> Cases_on `h0` >> gvs[is_halt_cml_def] >>
+      Cases_on `t` >> gvs[is_halt_cml_def]
+      )
+    )
+  >- (
+    pop_assum $ qspec_then `n` assume_tac >>
+    CCONTR_TAC >> gvs[is_halt_cml_def]
+    )
+  >- goal_assum drule
+QED
+
 Theorem application_not_Estuck:
   application op env st_ffi vs cs ≠ Estuck
 Proof
-  rw[smallStepTheory.application_def] >> EVERY_CASE_TAC >> gvs[SF smallstep_ss]
+  rw[cml_application_thm] >>
+  EVERY_CASE_TAC >> gvs[SF smallstep_ss]
 QED
 
 Theorem e_step_to_Estuck:
@@ -125,13 +268,13 @@ Proof
   reverse $ eq_tac
   >- (rw[] >> gvs[SF smallstep_ss]) >>
   gvs[e_step_def] >> CASE_TAC >> gvs[]
-  >- (EVERY_CASE_TAC >> gvs[SF smallstep_ss, application_not_Estuck]) >>
+  >- (every_case_tac >> gvs[SF smallstep_ss, application_not_Estuck]) >>
   Cases_on `cs` >> gvs[SF smallstep_ss] >>
-  EVERY_CASE_TAC >> gvs[application_not_Estuck]
+  every_case_tac >> gvs[application_not_Estuck]
 QED
 
 Theorem e_diverges_eq_step_to_halt_cml:
-  e_diverges env st_ffi e ⇔ step_to_halt_cml env st_ffi (Exp e) [] = NONE
+  e_diverges env st_ffi e ⇔ step_to_halt_cml (Estep (env, st_ffi, Exp e, [])) = NONE
 Proof
   rw[step_to_halt_cml_def, e_diverges_def, e_step_reln_eq_step_n_cml] >>
   simp[PULL_EXISTS] >>
@@ -216,38 +359,66 @@ Theorem application_rel:
 Proof
   rw[] >>
   drule do_app_rel >> disch_then $ qspecl_then [`vs`,`st`,`ffi`] assume_tac >>
-  rw[application_def, smallStepTheory.application_def] >>
+  rw[application_def, cml_application_thm]
+  >- (CASE_TAC >> gvs[step_result_rel_cases] >> CASE_TAC >> gvs[]) >>
+  Cases_on `do_app (st,ffi) op vs` >> gvs[] >>
+  Cases_on `do_app st op vs` >> gvs[]
+  >- (rpt (TOP_CASE_TAC >> gvs[step_result_rel_cases])) >>
+  gvs[FST_THM] >>
+  rpt (pairarg_tac >> gvs[]) >> gvs[result_rel_cases] >>
   rpt (
     TOP_CASE_TAC >>
-    gvs[step_result_rel_cases, result_rel_cases, ctxt_rel_def,
-        ctxt_frame_rel_cases, SF smallstep_ss, SF itree_ss]
-    ) >>
-  metis_tac[PAIR]
+    gvs[step_result_rel_cases, SF smallstep_ss, SF itree_ss,
+        ctxt_rel_def, ctxt_frame_rel_cases]
+    )
 QED
 
 Triviality application_FFI_results:
-  application (FFI s) env st vs cs = res ⇒
-  res = Etype_error ∨ ∃conf ws lnum. res = Effi s conf ws lnum env st cs
+  (application (FFI s) env st vs cs = Etype_error) ∨
+  (application (FFI s) env st vs cs = Estep (env, st, Val $ Conv NONE [], cs)) ∨
+  ∃conf ws lnum.
+    (application (FFI s) env st vs cs) = Effi s conf ws lnum env st cs
 Proof
-  rw[application_def] >> EVERY_CASE_TAC >> gvs[]
+  rw[application_def] >> every_case_tac >> gvs[]
 QED
 
 Theorem application_rel_FFI_type_error:
   application (FFI s) env st vs cs1 = Etype_error ⇔
   application (FFI s) env (st, ffi) vs cs2 = Eabort Rtype_error
 Proof
-  rw[application_def, smallStepTheory.application_def] >>
+  rw[application_def, cml_application_thm] >>
   simp[semanticPrimitivesTheory.do_app_def] >>
-  EVERY_CASE_TAC >> gvs[SF smallstep_ss] >>
+  every_case_tac >> gvs[SF smallstep_ss] >>
   gvs[store_lookup_def, store_assign_def, store_v_same_type_def]
+QED
+
+Theorem application_rel_FFI_step:
+  application (FFI s) env st vs cs1 = Estep (env, st, Val v, cs1) ⇔
+  application (FFI s) env (st, ffi) vs cs2 = Estep (env, (st,ffi), Val v, cs2)
+Proof
+  rw[application_def, cml_application_thm] >>
+  simp[semanticPrimitivesTheory.do_app_def] >>
+  every_case_tac >> gvs[SF smallstep_ss] >>
+  gvs[call_FFI_def, store_lookup_def, store_assign_def, store_v_same_type_def]
+  >- (eq_tac >> rw[] >> metis_tac[LUPDATE_SAME]) >>
+  every_case_tac >> gvs[] >> rw[] >> gvs[ffi_state_component_equality]
+QED
+
+Triviality application_eq_Effi_fields:
+  application op env st vs cs = Effi s conf ws lnum env' st' cs' ⇒
+  op = FFI s ∧ env = env' ∧ st = st' ∧ cs' = cs ∧
+  ∃conf'.
+    vs = [Litv $ StrLit conf'; Loc lnum] ∧
+    conf = MAP (λc. n2w $ ORD c) (EXPLODE conf')
+Proof
+  Cases_on `op` >> simp[application_def, SF itree_ss] >>
+  every_case_tac >> gvs[] >> rw[]
 QED
 
 Theorem application_rel_FFI:
   application (FFI s) env st vs cs1 = Effi s conf ws lnum env st cs1 ⇒
-  ∃ws.
     store_lookup lnum st = SOME $ W8array ws ∧
     application (FFI s) env (st, ffi) vs cs2 =
-      if s = "" then Estep (env, (st, ffi), Val $ Conv NONE [], cs2) else
       case ffi.oracle s ffi.ffi_state conf ws of
       | Oracle_return ffi' ws' =>
           if LENGTH ws' ≠ LENGTH ws then
@@ -266,27 +437,27 @@ Proof
   simp[application_def] >>
   ntac 6 (TOP_CASE_TAC >> gvs[]) >>
   gvs[store_lookup_def] >>
-  ntac 2 (TOP_CASE_TAC >> gvs[]) >> rw[] >>
-  goal_assum drule >>
+  ntac 2 (TOP_CASE_TAC >> gvs[]) >> rw[] >> gvs[] >>
   simp[smallStepTheory.application_def, semanticPrimitivesTheory.do_app_def] >>
   simp[store_lookup_def, call_FFI_def] >>
-  reverse IF_CASES_TAC >> gvs[store_assign_def, store_v_same_type_def]
-  >- (simp[SF smallstep_ss] >> drule LUPDATE_SAME >> gvs[]) >>
   qmatch_goalsub_abbrev_tac `foo l` >>
   reverse $ Cases_on `foo l` >> gvs[] >>
-  IF_CASES_TAC >> gvs[SF smallstep_ss]
+  IF_CASES_TAC >> gvs[store_assign_def, store_v_same_type_def, SF smallstep_ss]
 QED
 
 Theorem application_rel_FFI':
   application (FFI s) env (st, ffi) vs cs2 ≠ Eabort Rtype_error ⇒
-  ∃conf lnum ws.
+  (∃conf lnum ws.
     vs = [Litv $ StrLit conf; Loc lnum] ∧
     store_lookup lnum st = SOME $ W8array ws ∧
     application (FFI s) env st vs cs1 =
-      Effi s (MAP (λc. n2w $ ORD c) (EXPLODE conf)) ws lnum env st cs1
+      Effi s (MAP (λc. n2w $ ORD c) (EXPLODE conf)) ws lnum env st cs1) ∨
+  (s = "" ∧
+  application (FFI s) env st vs cs1 = Estep (env, st, Val $ Conv NONE [], cs1))
 Proof
   rw[smallStepTheory.application_def, semanticPrimitivesTheory.do_app_def] >>
-  EVERY_CASE_TAC >> gvs[application_def]
+  every_case_tac >> gvs[application_def] >>
+  IF_CASES_TAC >> gvs[]
 QED
 
 Theorem do_app_ffi_changed:
@@ -299,12 +470,18 @@ Theorem do_app_ffi_changed:
     s ≠ "" ∧
     ffi.oracle s ffi.ffi_state (MAP (λc. n2w $ ORD c) (EXPLODE conf)) ws =
       Oracle_return ffi_st ws' ∧
-    LENGTH ws = LENGTH ws'
+    LENGTH ws = LENGTH ws' ∧
+    st' = LUPDATE (W8array ws') lnum st ∧
+    ffi'.oracle = ffi.oracle ∧
+    ffi'.ffi_state = ffi_st ∧
+    ffi'.io_events =
+      ffi.io_events ++
+        [IO_event s (MAP (λc. n2w $ ORD c) (EXPLODE conf)) (ZIP (ws,ws'))]
 Proof
   simp[semanticPrimitivesTheory.do_app_def] >>
-  EVERY_CASE_TAC >> gvs[store_alloc_def, store_assign_def] >>
+  every_case_tac >> gvs[store_alloc_def, store_assign_def] >>
   strip_tac >> gvs[call_FFI_def] >>
-  EVERY_CASE_TAC >> gvs[]
+  every_case_tac >> gvs[]
 QED
 
 Theorem do_app_ffi_unchanged:
@@ -315,7 +492,7 @@ Theorem do_app_ffi_unchanged:
 Proof
   rpt gen_tac >>
   simp[semanticPrimitivesTheory.do_app_def] >>
-  EVERY_CASE_TAC >> gvs[store_alloc_def]
+  every_case_tac >> gvs[store_alloc_def]
 QED
 
 Theorem application_ffi_unchanged:
@@ -325,39 +502,48 @@ Theorem application_ffi_unchanged:
   ⇒ ffi = ffi'
 Proof
   rpt gen_tac >>
-  rw[smallStepTheory.application_def, SF smallstep_ss] >>
+  rw[cml_application_thm, SF smallstep_ss]
+  >- (every_case_tac >> gvs[]) >>
   qspecl_then [`st`,`ffi`,`op`,`vs`] assume_tac do_app_ffi_unchanged >>
-  EVERY_CASE_TAC >> gvs[]
+  every_case_tac >> gvs[]
 QED
 
 Theorem e_step_ffi_changed:
   e_step (env, (st, ffi), ev, cs) = Estep (env', (st', ffi'), ev', cs') ∧
   ffi ≠ ffi' ⇒
-  ∃ s conf lnum env'' ccs ws ffi_st ws'.
+  ∃ s conf lnum ccs ws ffi_st ws'.
     ev = Val (Litv (StrLit conf)) ∧
-    cs = (Capp (FFI s) [Loc lnum] () [], env'') :: ccs ∧
+    cs = (Capp (FFI s) [Loc lnum] () [], env') :: ccs ∧
     store_lookup lnum st = SOME (W8array ws) ∧
     s ≠ "" ∧
     ffi.oracle s ffi.ffi_state (MAP (λc. n2w $ ORD c) (EXPLODE conf)) ws =
       Oracle_return ffi_st ws' ∧
-    LENGTH ws = LENGTH ws'
+    LENGTH ws = LENGTH ws' ∧
+    ev' = Val (Conv NONE []) ∧
+    cs' = ccs ∧
+    st' = LUPDATE (W8array ws') lnum st ∧
+    ffi'.oracle = ffi.oracle ∧
+    ffi'.ffi_state = ffi_st ∧
+    ffi'.io_events =
+      ffi.io_events ++
+        [IO_event s (MAP (λc. n2w $ ORD c) (EXPLODE conf)) (ZIP (ws,ws'))]
 Proof
   simp[e_step_def] >>
-  EVERY_CASE_TAC >> gvs[SF smallstep_ss]
+  every_case_tac >> gvs[SF smallstep_ss]
   >- (
     strip_tac >> rename1 `application op _ _ _ _` >>
     Cases_on `∀s. op ≠ FFI s` >> gvs[]
     >- (irule application_ffi_unchanged >> rpt $ goal_assum drule) >>
     gvs[smallStepTheory.application_def, semanticPrimitivesTheory.do_app_def]
     ) >>
-  EVERY_CASE_TAC >> gvs[] >>
+  every_case_tac >> gvs[] >>
   rename1 `application op _ _ _ _` >>
   (
     strip_tac >> Cases_on `∀s. op ≠ FFI s` >> gvs[]
     >- (drule_all application_ffi_unchanged >> gvs[]) >>
     gvs[smallStepTheory.application_def,
         semanticPrimitivesTheory.do_app_def, call_FFI_def] >>
-    EVERY_CASE_TAC >> gvs[SF smallstep_ss]
+    every_case_tac >> gvs[SF smallstep_ss, store_lookup_def, store_assign_def]
   )
 QED
 
@@ -377,6 +563,160 @@ Definition trace_prefix_def:
         (IO_event s conf (ZIP (ws,ws'))::io, res)
     | Oracle_final outcome => trace_prefix n (oracle, st) (f $ INL outcome)
 End
+
+Definition is_Effi_def:
+  is_Effi (Effi _ _ _ _ _ _ _) = T ∧
+  is_Effi _ = F
+End
+
+Theorem is_Effi_def:
+  is_Effi e ⇔ ∃ s ws1 ws2 n env st cs. e = Effi s ws1 ws2 n env st cs
+Proof
+  Cases_on `e` >> simp[is_Effi_def]
+QED
+
+Definition get_ffi_def:
+  get_ffi (Estep (env, (st, ffi), ev, cs)) = SOME ffi ∧
+  get_ffi _ = NONE
+End
+
+Theorem step_result_rel_single:
+  ∀ea eb.
+    step_result_rel (Estep ea) (Estep eb) ∧
+    ¬ is_Effi (estep ea)
+  ⇒ step_result_rel (estep ea) (e_step eb) ∧
+    ∀ffi. get_ffi (e_step eb) = SOME ffi ⇒ get_ffi (Estep eb) = SOME ffi
+Proof
+  rpt PairCases >> rename1 `_ (_ (env,st,ev,cs1)) (_ (env',(st',ffi),ev',cs2))` >>
+  gvs[e_step_def] >>
+  every_case_tac >> gvs[estep_def, step_result_rel_cases] >> strip_tac >>
+  gvs[SF smallstep_ss, SF itree_ss, ctxt_rel_def, ctxt_frame_rel_cases, get_ffi_def] >>
+  gvs[GSYM ctxt_frame_rel_cases, GSYM step_result_rel_cases]
+  >- (
+    rename1 `application op _ _ _ _` >>
+    reverse $ Cases_on `∃s. op = FFI s` >> gvs[]
+    >- (
+      reverse $ rw[]
+      >- (
+        drule application_ffi_unchanged >>
+        Cases_on `application op env (st,ffi) [] cs2` >> gvs[get_ffi_def] >>
+        PairCases_on `p` >> disch_then drule >> gvs[get_ffi_def]
+        )
+      >- (
+        drule application_rel >> gvs[ctxt_rel_def] >> disch_then drule >>
+        disch_then $ qspecl_then [`[]`,`st`,`ffi`,`env`] assume_tac >>
+        gvs[step_result_rel_cases, ctxt_rel_def]
+        )
+      ) >>
+    qspecl_then [`[]`,`st`,`s`,`env`,`cs1`]
+      assume_tac $ GEN_ALL application_FFI_results >> gvs[] >>
+    csimp[] >> gvs[is_Effi_def, get_ffi_def]
+    >- metis_tac[application_rel_FFI_type_error] >>
+    imp_res_tac application_rel_FFI_step >> simp[get_ffi_def]
+    )
+  >- gvs[FST_THM, LAMBDA_PROD]
+  >- gvs[FST_THM, LAMBDA_PROD] >>
+  CASE_TAC >- gvs[continue_def, get_ffi_def] >>
+  PairCases_on `h` >> gvs[] >> PairCases_on `x` >> gvs[] >>
+  rename1 `ctxt_frame_rel c1 c2` >> rename1 `(c1,env)` >>
+  rename1 `LIST_REL _ rest1 rest2` >>
+  Cases_on `c1` >> gvs[SF itree_ss, ctxt_frame_rel_cases] >>
+  gvs[GSYM ctxt_frame_rel_cases, get_ffi_def]
+  >- (EVERY_CASE_TAC >> gvs[get_ffi_def, ctxt_frame_rel_cases])
+  >- (
+    reverse CASE_TAC >>
+    gvs[PULL_EXISTS, EXISTS_PROD, get_ffi_def, SF itree_ss]
+    >- simp[ctxt_frame_rel_cases] >>
+    rename1 `application op _ _ vs _` >>
+    reverse $ Cases_on `∃s. op = FFI s` >> gvs[]
+    >- (
+      reverse $ rw[]
+      >- (
+        drule application_ffi_unchanged >>
+        Cases_on `application op env (st,ffi) vs rest2` >> gvs[get_ffi_def] >>
+        PairCases_on `p` >> disch_then drule >> gvs[get_ffi_def]
+        )
+      >- (
+        drule application_rel >> gvs[ctxt_rel_def] >> disch_then drule >>
+        disch_then $ qspecl_then [`vs`,`st`,`ffi`,`env`] assume_tac >>
+        gvs[step_result_rel_cases, ctxt_rel_def]
+        )
+      ) >>
+    qspecl_then [`vs`,`st`,`s`,`env`,`rest1`]
+      assume_tac $ GEN_ALL application_FFI_results >> gvs[] >>
+    csimp[] >> gvs[is_Effi_def, get_ffi_def]
+    >- metis_tac[application_rel_FFI_type_error] >>
+    imp_res_tac application_rel_FFI_step >> gvs[get_ffi_def]
+    )
+  >- (EVERY_CASE_TAC >> gvs[get_ffi_def, ctxt_frame_rel_cases])
+  >- (EVERY_CASE_TAC >> gvs[get_ffi_def, ctxt_frame_rel_cases])
+  >- (EVERY_CASE_TAC >> gvs[get_ffi_def, ctxt_frame_rel_cases])
+  >- (
+    CASE_TAC >> gvs[PULL_EXISTS, EXISTS_PROD, get_ffi_def, SF itree_ss]
+    >- simp[ctxt_frame_rel_cases] >>
+    CASE_TAC >>  gvs[SF itree_ss] >>
+    EVERY_CASE_TAC >> gvs[get_ffi_def, ctxt_frame_rel_cases]
+    )
+  >- (
+    TOP_CASE_TAC >> gvs[SF itree_ss] >>
+    EVERY_CASE_TAC >> gvs[get_ffi_def, ctxt_frame_rel_cases]
+    )
+QED
+
+Theorem step_result_rel_n:
+  ∀n ea eb.
+    step_result_rel ea eb ∧
+    ¬ is_Effi (step_n n ea)
+  ⇒ step_result_rel (step_n n ea) (step_n_cml n eb) ∧
+    ∀ffi. get_ffi (step_n_cml n eb) = SOME ffi ⇒ get_ffi eb = SOME ffi
+Proof
+  Induct >- simp[step_n_def, step_n_cml_def] >>
+  simp[step_n_alt_def, step_n_cml_alt_def] >>
+  rpt gen_tac >> strip_tac >>
+  last_x_assum drule >> impl_keep_tac
+  >- (CCONTR_TAC >> gvs[is_Effi_def]) >>
+  strip_tac >>
+  Cases_on `step_n n ea` >> imp_res_tac step_result_rel_cases >> gvs[get_ffi_def] >>
+  simp[GSYM step_result_rel_cases] >>
+  qmatch_goalsub_abbrev_tac `step_result_rel (estep ea) (e_step eb)` >>
+  qspecl_then [`ea`,`eb`] assume_tac step_result_rel_single >> gvs[] >>
+  unabbrev_all_tac >> gvs[get_ffi_def]
+QED
+
+Theorem step_result_rel_single_FFI:
+  ∀ea eb.
+    step_result_rel (Estep ea) (Estep eb) ∧
+    estep ea = Effi s ws1 ws2 lnum env' st' cs1'
+  ⇒ ∃ffi.
+      get_ffi (Estep eb) = SOME ffi ∧
+      ((∃ffi'. get_ffi (e_step eb) = SOME ffi' ∧ ffi' ≠ ffi)  ∨
+       (∃outcome. e_step eb = Eabort (Rffi_error (Final_event s ws1 ws2 outcome))))
+Proof
+  rpt PairCases >> gvs[step_result_rel_cases, e_step_def] >> rw[] >>
+  rename1 `estep (env,st,ev,cs1)` >> rename1 `Estep ((env,(st,ffi),ev,cs2))` >>
+  gvs[get_ffi_def] >>
+  every_case_tac >> gvs[estep_def, step_result_rel_cases, FST_THM, LAMBDA_PROD] >>
+  gvs[SF smallstep_ss, SF itree_ss, ctxt_rel_def, ctxt_frame_rel_cases, get_ffi_def]
+  >- (imp_res_tac application_eq_Effi_fields >> gvs[application_def, SF itree_ss]) >>
+  TOP_CASE_TAC >> gvs[SF itree_ss] >>
+  pairarg_tac >> gvs[] >>
+  pairarg_tac >> gvs[get_ffi_def, SF itree_ss]
+  >- (EVERY_CASE_TAC >> gvs[])
+  >- (
+    CASE_TAC >> gvs[SF itree_ss, GSYM ctxt_frame_rel_cases] >>
+    imp_res_tac application_eq_Effi_fields >> gvs[] >>
+    rename [`LIST_REL _ cs1 cs2`, `application _ env`] >>
+    drule application_rel_FFI >>
+    disch_then $ qspecl_then [`ffi`,`cs2`] assume_tac >> gvs[] >>
+    every_case_tac >> gvs[get_ffi_def] >>
+    gvs[ffi_state_component_equality]
+    )
+  >- (EVERY_CASE_TAC >> gvs[])
+  >- (EVERY_CASE_TAC >> gvs[])
+  >- (EVERY_CASE_TAC >> gvs[])
+  >- (rpt (CASE_TAC >> gvs[SF itree_ss]))
+  >- (rpt (CASE_TAC >> gvs[SF itree_ss]))
+QED
 
 
 (****************************************)
